Fixed the definition of the semantics of C module

compcertox/CModule.v
@@ -2,7 +2,7 @@ Require Import Relations RelationClasses Relators.
 Require Import List Maps.
 Require Import Coqlib.
 Require Import CallconvAlgebra_.
-Require Import LanguageInterface_ Events Globalenvs Smallstep_ CategoricalComp FlatComp.
+Require Import LanguageInterface_ Events Globalenvs Smallstep_ CategoricalComp FlatComp SmallstepLinking_.
 Require Import Memory Values.
 Require Import Clight_ Linking.
 Require Import AbstractStateRel Lifting.
@@ -19,171 +19,343 @@ Require Import Ctypes.
    Clight programs *)
 Notation cmodule := (list Clight_.program).
 
-(* For some reason p ⊕ id can't be simply replaced by p *)
-(* The patterns are overlapping because Coq is not able to find the termination
-   order automatically *)
-Fixpoint semantics (cmod: cmodule) sk: semantics li_c li_c :=
-  match cmod with
-  | nil => id_semantics sk
-  | (p :: nil) => skel_extend (Clight_.semantics1 p) sk
-  | (p :: ps) =>
-    let L b := match b with
-               | true  => skel_extend (Clight_.semantics1 p) sk
-               | false => semantics ps sk
-               end
-    in SmallstepLinking_.semantics L sk
+Fixpoint pos (M: cmodule): Type :=
+  match M with
+  | nil => Empty_set
+  | p :: ps => unit + pos ps
   end.
 
-Section LIST_IND.
-  Variable A: Type.
-  Variable P: list A -> Prop.
-  Variable P1: forall x, P (x :: nil).
-  Variable Pcons: forall x xs, P xs -> P (x :: xs).
+Definition ref (M: cmodule) (k: pos M): Smallstep_.semantics li_c li_c.
+Proof.
+  induction M as [| p ps].
+  - inv k.
+  - destruct k.
+    + refine (Clight_.semantics1 p).
+    + apply IHps. apply p0.
+Defined.
 
-  Theorem list_ind1: forall xs, (List.length xs >= 1)%nat -> P xs.
-  Proof.
-    set (Q := fun l => (Datatypes.length l >= 1)%nat -> P l).
-    apply (@list_ind A Q).
-    - unfold Q. inversion 1.
-    - subst Q. cbn. intros.
-      destruct l.
-      + apply P1.
-      + apply Pcons. apply H. cbn. firstorder.
-  Qed.
-End LIST_IND.
+Definition semantics (M: cmodule) sk: Smallstep_.semantics li_c li_c :=
+  SmallstepLinking_.semantics' (ref M) sk.
 
-Definition skel_module_compatible (sk: AST.program unit unit) (M: cmodule) :=
-  Forall (fun (p: Clight_.program) => linkorder (AST.erase_program p) sk) M.
+Require Import FunctionalExtensionality.
+Require Import FinFun.
 
-Section HCOMP_STATE.
-  Context {li} (L1 L2: Smallstep_.semantics li li).
-  Let L := fun i => match i with | true => L1 | false => L2 end.
-
-  Lemma initial_state_valid_comp sk:
-    forall q s se,
-      Smallstep_.initial_state (SmallstepLinking_.semantics L sk se) q s ->
-      valid_query (SmallstepLinking_.semantics L sk) se q.
-  Proof.
-    intros q s se Hx. inv Hx. destruct i; firstorder.
-  Qed.
-
-  Lemma extcall_invalid_comp sk:
-    forall q s se,
-      Smallstep_.at_external (SmallstepLinking_.semantics L sk se) s q ->
-      ~ valid_query (SmallstepLinking_.semantics L sk) se q.
-  Proof.
-    intros q s se Hx. inv Hx. destruct i.
-    - intros (?&?&Hfp&?). destruct Hfp.
-      + apply (H0 true). firstorder.
-      + apply (H0 false). firstorder.
-    - intros (?&?&Hfp&?). destruct Hfp.
-      + apply (H0 true). firstorder.
-      + apply (H0 false). firstorder.
-  Qed.
-
-End HCOMP_STATE.
-
-(* Overlapping patterns in the definition of semantics results in duplicate
-   proofs *)
 Lemma cmodule_initial_state_valid sk M:
-  (List.length M >= 1)%nat ->
   forall se s q, Smallstep_.initial_state (semantics M sk se) q s ->
             valid_query (semantics M sk) se q.
 Proof.
-  set (P := fun M => forall se s q, Smallstep_.initial_state (semantics M sk se) q s -> valid_query (semantics M sk) se q).
-  apply (@list_ind1 _ P); subst P; cbn beta.
-  - intros. eapply initial_state_valid; eauto.
-  (* inv H. destruct H0 as (? & ? & ? & ?). destruct i. *)
-  (* + unfold valid_query. split; auto. *)
-  (*   eexists; split; eauto. now left. *)
-  (* + inv H0. *)
-  - intros p ps IH se s q H. cbn. destruct ps as [| p' ps'].
-    + eapply initial_state_valid; eauto.
-    + eapply initial_state_valid_comp. apply H.
+  intros. inv H. destruct H0 as (?&?&?&?).
+  split; eauto.
+  eexists; split; eauto.
+  cbn. eexists; eauto.
 Qed.
 
-Lemma cmodule_extcall_invalid sk M:
-  (List.length M >= 1)%nat ->
-  forall se s q, Smallstep_.at_external (semantics M sk se) s q ->
-            ~ valid_query (semantics M sk) se q.
+Section APP.
+
+  Context (M N: cmodule).
+  Variable (sk: AST.program unit unit).
+
+  Let L := fun (b: bool) => match b with | true => (semantics M sk) | false => (semantics N sk) end.
+  Let J := fun (b: bool) => match b with | true => pos M | false => pos N end.
+  Definition Lij: forall (b: bool), J b -> Smallstep_.semantics li_c li_c.
+  Proof.
+    intros [|] j.
+    - refine (ref M j).
+    - refine (ref N j).
+  Defined.
+
+  Lemma Leq: L = (fun i => semantics' (fun j => Lij i j) sk).
+  Proof.
+    apply functional_extensionality. intros [|]; reflexivity.
+  Qed.
+
+  Definition F: pos (M ++ N) -> {b : bool & J b}.
+  Proof.
+    intros x. induction M as [| p ps].
+    - refine (existT _ false x).
+    - cbn in *. destruct x.
+      + refine (existT _ true (inl u)).
+      + specialize (IHps p0) as [[|] pp].
+        * refine (existT _ true (inr pp)).
+        * refine (existT _ false pp).
+  Defined.
+
+  Definition G: {b : bool & J b} -> pos (M ++ N).
+  Proof.
+    intros [[|] j].
+    - cbn in *. induction M as [| p ps].
+      + inv j.
+      + cbn. destruct j.
+        * refine (inl u).
+        * refine (inr (IHps p0)).
+    - cbn in *. induction M as [| p ps].
+      + refine j.
+      + refine (inr IHps).
+  Defined.
+
+  Lemma FG_bij: Bijective F.
+  Proof.
+    exists G. split; intros x.
+    - unfold F, G. cbn.
+      induction M as [| p ps].
+      + reflexivity.
+      + cbn in *. destruct x.
+        * reflexivity.
+        * cbn in *. specialize (IHps p0).
+          remember (list_rect (fun l : cmodule => pos (l ++ N) -> _) _ _ ps p0) as lr.
+          destruct lr as [b pb]. destruct b.
+          -- f_equal. apply IHps.
+          -- f_equal. apply IHps.
+    - unfold F, G. cbn. destruct x as [[|] j].
+      + cbn in *. induction M as [| p ps].
+        * cbn in *. inv j.
+        * cbn in *. destruct j.
+          -- constructor.
+          -- specialize (IHps p0). cbn in *.
+             rewrite IHps. constructor.
+      + cbn in *. induction M as [| p ps].
+        * cbn in *. constructor.
+        * cbn in *. rewrite IHps. constructor.
+  Qed.
+
+  Lemma LFeq: (fun i : pos (M ++ N) => (fun p : {x : bool & J x} => Lij (projT1 p) (projT2 p)) (F i)) = ref (M ++ N).
+  Proof.
+    apply functional_extensionality. intros x.
+    unfold F, Lij. induction M as [| p ps].
+    - cbn in *. reflexivity.
+    - cbn in *. destruct x.
+      + reflexivity.
+      + cbn in *. specialize (IHps p0).
+        remember (list_rect (fun l : cmodule => pos (l ++ N) -> _) _ _ ps p0) as lr.
+        destruct lr as [b pb]. destruct b.
+        * cbn in *. apply IHps.
+        * cbn in *. apply IHps.
+  Qed.
+
+  Lemma cmodule_app_simulation:
+    comp_semantics' (semantics M sk) (semantics N sk) sk ≤ semantics (M ++ N) sk.
+  Proof.
+    etransitivity.
+    {
+      apply categorical_compose_approximation.
+      intros [|] se q s H.
+      eapply cmodule_initial_state_valid; eauto.
+      eapply cmodule_initial_state_valid; eauto.
+    }
+    fold L. rewrite Leq.
+    etransitivity. apply level_simulation1.
+    etransitivity. eapply bijective_map_simulation1 with (F := F).
+    apply FG_bij. unfold semantics. rewrite <- LFeq.
+    (* FIXME: add typeclass *)
+    apply identity_forward_simulation.
+  Qed.
+
+End APP.
+
+Definition skel_module_compatible (M: cmodule) (sk: AST.program unit unit) :=
+  Forall (fun (p: Clight_.program) => linkorder (AST.erase_program p) sk) M.
+
+Lemma cmodule_krel {K1 K2} (R: rel_adt K1 K2) M sk:
+  skel_module_compatible M sk ->
+  forward_simulation R R (semantics M sk @ K1) (semantics M sk @ K2).
 Proof.
-  set (P := fun M =>  forall se s q, Smallstep_.at_external ((semantics M sk) se) s q -> ~ valid_query (semantics M sk) se q).
-  apply (@list_ind1 _ P); subst P; cbn beta.
-  - intros. eapply extcall_invalid; eauto.
-  - intros p ps IH se s q H. destruct ps as [| p' ps'].
-    + eapply extcall_invalid; eauto.
-    + eapply extcall_invalid_comp. apply H.
+  intros Hsk.
+
+  eapply open_fsim_ccref. apply cc_compose_id_left.
+  unfold flip. apply cc_compose_id_left.
+  eapply compose_forward_simulations.
+  apply lift_horizontal_comp1.
+
+  eapply open_fsim_ccref. apply cc_compose_id_right.
+  unfold flip. apply cc_compose_id_right.
+  eapply compose_forward_simulations.
+  2: { apply lift_horizontal_comp2. }
+
+  apply horizontal_compose_simulation'.
+  - intros. induction M as [| p ps]; try easy.
+    destruct i.
+    + cbn. apply clight_krel.
+    + apply IHps.
+      unfold skel_module_compatible in *.
+      rewrite -> Forall_forall in *.
+      intros x Hx. apply Hsk. right. auto.
+  - intros. induction M as [| p ps]; try easy.
+    destruct i.
+    + cbn. unfold skel_module_compatible in *.
+      rewrite -> Forall_forall in *. apply Hsk.
+      left. auto.
+    + apply IHps.
+      unfold skel_module_compatible in *.
+      rewrite -> Forall_forall in *.
+      intros x Hx. apply Hsk. right. auto.
 Qed.
+
+(* Legacy definition of C module and related proof *)
+
+(* For some reason p ⊕ id can't be simply replaced by p *)
+(* The patterns are overlapping because Coq is not able to find the termination
+   order automatically *)
+
+(* Fixpoint semantics (cmod: cmodule) sk: semantics li_c li_c := *)
+(*   match cmod with *)
+(*   | nil => id_semantics sk *)
+(*   | (p :: nil) => skel_extend (Clight_.semantics1 p) sk *)
+(*   | (p :: ps) => *)
+(*     let L b := match b with *)
+(*                | true  => skel_extend (Clight_.semantics1 p) sk *)
+(*                | false => semantics ps sk *)
+(*                end *)
+(*     in SmallstepLinking_.semantics L sk *)
+(*   end. *)
+
+(* Section LIST_IND. *)
+(*   Variable A: Type. *)
+(*   Variable P: list A -> Prop. *)
+(*   Variable P1: forall x, P (x :: nil). *)
+(*   Variable Pcons: forall x xs, P xs -> P (x :: xs). *)
+
+(*   Theorem list_ind1: forall xs, (List.length xs >= 1)%nat -> P xs. *)
+(*   Proof. *)
+(*     set (Q := fun l => (Datatypes.length l >= 1)%nat -> P l). *)
+(*     apply (@list_ind A Q). *)
+(*     - unfold Q. inversion 1. *)
+(*     - subst Q. cbn. intros. *)
+(*       destruct l. *)
+(*       + apply P1. *)
+(*       + apply Pcons. apply H. cbn. firstorder. *)
+(*   Qed. *)
+(* End LIST_IND. *)
+
+(* Section HCOMP_STATE. *)
+(*   Context {li} (L1 L2: Smallstep_.semantics li li). *)
+(*   Let L := fun i => match i with | true => L1 | false => L2 end. *)
+
+(*   Lemma initial_state_valid_comp sk: *)
+(*     forall q s se, *)
+(*       Smallstep_.initial_state (SmallstepLinking_.semantics L sk se) q s -> *)
+(*       valid_query (SmallstepLinking_.semantics L sk) se q. *)
+(*   Proof. *)
+(*     intros q s se Hx. inv Hx. destruct i; firstorder. *)
+(*   Qed. *)
+
+(*   Lemma extcall_invalid_comp sk: *)
+(*     forall q s se, *)
+(*       Smallstep_.at_external (SmallstepLinking_.semantics L sk se) s q -> *)
+(*       ~ valid_query (SmallstepLinking_.semantics L sk) se q. *)
+(*   Proof. *)
+(*     intros q s se Hx. inv Hx. destruct i. *)
+(*     - intros (?&?&Hfp&?). destruct Hfp. *)
+(*       + apply (H0 true). firstorder. *)
+(*       + apply (H0 false). firstorder. *)
+(*     - intros (?&?&Hfp&?). destruct Hfp. *)
+(*       + apply (H0 true). firstorder. *)
+(*       + apply (H0 false). firstorder. *)
+(*   Qed. *)
+
+(* End HCOMP_STATE. *)
+
+(* Overlapping patterns in the definition of semantics results in duplicate
+   proofs *)
+
+(* Lemma cmodule_initial_state_valid sk M: *)
+(*   (List.length M >= 1)%nat -> *)
+(*   forall se s q, Smallstep_.initial_state (semantics M sk se) q s -> *)
+(*             valid_query (semantics M sk) se q. *)
+(* Proof. *)
+(*   set (P := fun M => forall se s q, Smallstep_.initial_state (semantics M sk se) q s -> valid_query (semantics M sk) se q). *)
+(*   apply (@list_ind1 _ P); subst P; cbn beta. *)
+(*   - intros. eapply initial_state_valid; eauto. *)
+(*   (* inv H. destruct H0 as (? & ? & ? & ?). destruct i. *) *)
+(*   (* + unfold valid_query. split; auto. *) *)
+(*   (*   eexists; split; eauto. now left. *) *)
+(*   (* + inv H0. *) *)
+(*   - intros p ps IH se s q H. cbn. destruct ps as [| p' ps']. *)
+(*     + eapply initial_state_valid; eauto. *)
+(*     + eapply initial_state_valid_comp. apply H. *)
+(* Qed. *)
+
+(* Lemma cmodule_extcall_invalid sk M: *)
+(*   (List.length M >= 1)%nat -> *)
+(*   forall se s q, Smallstep_.at_external (semantics M sk se) s q -> *)
+(*             ~ valid_query (semantics M sk) se q. *)
+(* Proof. *)
+(*   set (P := fun M =>  forall se s q, Smallstep_.at_external ((semantics M sk) se) s q -> ~ valid_query (semantics M sk) se q). *)
+(*   apply (@list_ind1 _ P); subst P; cbn beta. *)
+(*   - intros. eapply extcall_invalid; eauto. *)
+(*   - intros p ps IH se s q H. destruct ps as [| p' ps']. *)
+(*     + eapply extcall_invalid; eauto. *)
+(*     + eapply extcall_invalid_comp. apply H. *)
+(* Qed. *)
 
 
 (* M has to be non-empty is due to the fact that we can't prove id ∘ L ≡ L *)
 (* No, the reason is the id LTS doesn't have initial_state_valid *)
-Lemma cmodule_simulation {M N : cmodule} {sk: AST.program unit unit}:
-  (List.length N >= 1)%nat -> (List.length M >= 1)%nat ->
-  comp_semantics' (semantics M sk) (semantics N sk) sk ≤ semantics (M ++ N) sk.
-Proof.
-  intros HN HM. etransitivity.
-  - apply categorical_compose_approximation.
-    intros [|] se q s H.
-    eapply cmodule_initial_state_valid; eauto.
-    eapply cmodule_initial_state_valid; eauto.
-  - induction M as [|p ps].
-    + cbn. etransitivity; [ | apply hcomp_left_identity1 ].
-      assert (skel (semantics N sk) = sk).
-      { destruct N; auto. destruct N; auto. }
-      rewrite H. apply identity_forward_simulation.
-      apply cmodule_extcall_invalid; auto.
-    + rewrite <- app_comm_cons. destruct ps as [| p' ps'].
-      * destruct N as [| q qs].
-        -- apply hcomp_right_identity1.
-           apply extcall_invalid.
-           intros. exploit initial_state_valid.
-           apply H. intros Hx. apply Hx.
-        -- apply horizontal_compose_simulation'.
-           ++ apply identity_forward_simulation.
-           ++ fold semantics. apply identity_forward_simulation.
-           ++ apply linkorder_refl.
-           ++ destruct qs; apply linkorder_refl.
-      * edestruct IHps. cbn. omega.
-        set (ps := p' :: ps') in *. clear IHps.
-        etransitivity.
-        -- apply horizontal_compose_associativity.
-        -- fold semantics.
-           apply horizontal_compose_simulation'.
-           ++ apply identity_forward_simulation.
-           ++ fold semantics. constructor. apply X.
-           ++ apply linkorder_refl.
-           ++ apply linkorder_refl.
-Qed.
+(* Lemma cmodule_simulation {M N : cmodule} {sk: AST.program unit unit}: *)
+(*   (List.length N >= 1)%nat -> (List.length M >= 1)%nat -> *)
+(*   comp_semantics' (semantics M sk) (semantics N sk) sk ≤ semantics (M ++ N) sk. *)
+(* Proof. *)
+(*   intros HN HM. etransitivity. *)
+(*   - apply categorical_compose_approximation. *)
+(*     intros [|] se q s H. *)
+(*     eapply cmodule_initial_state_valid; eauto. *)
+(*     eapply cmodule_initial_state_valid; eauto. *)
+(*   - induction M as [|p ps]. *)
+(*     + cbn. etransitivity; [ | apply hcomp_left_identity1 ]. *)
+(*       assert (skel (semantics N sk) = sk). *)
+(*       { destruct N; auto. destruct N; auto. } *)
+(*       rewrite H. apply identity_forward_simulation. *)
+(*       apply cmodule_extcall_invalid; auto. *)
+(*     + rewrite <- app_comm_cons. destruct ps as [| p' ps']. *)
+(*       * destruct N as [| q qs]. *)
+(*         -- apply hcomp_right_identity1. *)
+(*            apply extcall_invalid. *)
+(*            intros. exploit initial_state_valid. *)
+(*            apply H. intros Hx. apply Hx. *)
+(*         -- apply horizontal_compose_simulation'. *)
+(*            ++ apply identity_forward_simulation. *)
+(*            ++ fold semantics. apply identity_forward_simulation. *)
+(*            ++ apply linkorder_refl. *)
+(*            ++ destruct qs; apply linkorder_refl. *)
+(*       * edestruct IHps. cbn. omega. *)
+(*         set (ps := p' :: ps') in *. clear IHps. *)
+(*         etransitivity. *)
+(*         -- apply horizontal_compose_associativity. *)
+(*         -- fold semantics. *)
+(*            apply horizontal_compose_simulation'. *)
+(*            ++ apply identity_forward_simulation. *)
+(*            ++ fold semantics. constructor. apply X. *)
+(*            ++ apply linkorder_refl. *)
+(*            ++ apply linkorder_refl. *)
+(* Qed. *)
 
-Lemma cmodule_krel {K1 K2} (R: rel_adt K1 K2) M sk:
-  (List.length M >= 1)%nat -> skel_module_compatible sk M ->
-  forward_simulation R R (semantics M sk @ K1) (semantics M sk @ K2).
-Proof.
-  set (P := fun M => skel_module_compatible sk M ->
-                  forward_simulation R R (semantics M sk @ K1) (semantics M sk @ K2)).
-  apply (@list_ind1 _ P); subst P; cbn beta.
-  - intros p Hsk. apply lift_skel_extend. apply clight_krel. now inv Hsk.
-  - intros p ps Hp Hsk.
-    destruct ps as [| p' ps'].
-    + apply lift_skel_extend. apply clight_krel. now inv Hsk.
-    + set (p' :: ps') as ps in *.
-      eapply open_fsim_ccref. apply cc_compose_id_left.
-      unfold flip. apply cc_compose_id_left.
-      eapply compose_forward_simulations.
-      apply lift_horizontal_comp1.
+(* Lemma cmodule_krel {K1 K2} (R: rel_adt K1 K2) M sk: *)
+(*   (List.length M >= 1)%nat -> skel_module_compatible sk M -> *)
+(*   forward_simulation R R (semantics M sk @ K1) (semantics M sk @ K2). *)
+(* Proof. *)
+(*   set (P := fun M => skel_module_compatible sk M -> *)
+(*                   forward_simulation R R (semantics M sk @ K1) (semantics M sk @ K2)). *)
+(*   apply (@list_ind1 _ P); subst P; cbn beta. *)
+(*   - intros p Hsk. apply lift_skel_extend. apply clight_krel. now inv Hsk. *)
+(*   - intros p ps Hp Hsk. *)
+(*     destruct ps as [| p' ps']. *)
+(*     + apply lift_skel_extend. apply clight_krel. now inv Hsk. *)
+(*     + set (p' :: ps') as ps in *. *)
+(*       eapply open_fsim_ccref. apply cc_compose_id_left. *)
+(*       unfold flip. apply cc_compose_id_left. *)
+(*       eapply compose_forward_simulations. *)
+(*       apply lift_horizontal_comp1. *)
 
-      fold semantics.
-      eapply open_fsim_ccref. apply cc_compose_id_right.
-      unfold flip. apply cc_compose_id_right.
-      eapply compose_forward_simulations.
-      2: { apply lift_horizontal_comp2. }
+(*       fold semantics. *)
+(*       eapply open_fsim_ccref. apply cc_compose_id_right. *)
+(*       unfold flip. apply cc_compose_id_right. *)
+(*       eapply compose_forward_simulations. *)
+(*       2: { apply lift_horizontal_comp2. } *)
 
-      fold semantics.
-      apply horizontal_compose_simulation'.
-      * apply lift_skel_extend. apply clight_krel. now inv Hsk.
-      * apply Hp. now inv Hsk.
-      * apply linkorder_refl.
-      * destruct ps. apply linkorder_refl.
-        destruct ps; apply linkorder_refl.
-Qed.
+(*       fold semantics. *)
+(*       apply horizontal_compose_simulation'. *)
+(*       * apply lift_skel_extend. apply clight_krel. now inv Hsk. *)
+(*       * apply Hp. now inv Hsk. *)
+(*       * apply linkorder_refl. *)
+(*       * destruct ps. apply linkorder_refl. *)
+(*         destruct ps; apply linkorder_refl. *)
+(* Qed. *)
