compcertox/CompCertO.v
@@ -8,51 +8,87 @@ Require Import LanguageInterface_ Events Globalenvs Smallstep_ CategoricalComp F
 Require Import Memory Values.
 Require Import Linking.
 
-Global Instance fsim_transitive {li1 li2: language_interface}:
-  Transitive (forward_simulation (@cc_id li1) (@cc_id li2)).
-Proof.
-  intros L1 L2 L3 HL1 HL2.
-  eapply open_fsim_ccref. apply cc_compose_id_left.
-  unfold flip. apply cc_compose_id_left.
-  eapply compose_forward_simulations; eauto.
-Qed.
 
+(* Lemma inhabited_ind_dep {I: Type} {X: I -> Type} {P: Prop}: (forall i, X i -> P) -> (forall i, inhabited (X i)) -> P. *)
+(* Proof. *)
+(*   intros f Hf. *)
+(* Admitted. *)
+
+(* I believe the above induction principle is provable, so we don't really
+   need the epsilon operator. Epsilon is more handy though *)
+Require Import ClassicalEpsilon.
 
 Section HCOMP_FSIM.
 
   Context {li1 li2} (cc: callconv li1 li2)
-          (L1a L1b: Smallstep_.semantics li1 li1)
-          (L2a L2b: Smallstep_.semantics li2 li2).
-  Hypothesis (HL1: forward_simulation cc cc L1a L2a)
-             (HL2: forward_simulation cc cc L1b L2b).
-  Let L1 := fun b => match b with | true => L1a | false => L1b end.
-  Let L2 := fun b => match b with | true => L2a | false => L2b end.
+          {I} (L1: I -> Smallstep_.semantics li1 li1)
+          (L2: I -> Smallstep_.semantics li2 li2).
 
+  Hypothesis (H: forall i, forward_simulation cc cc (L1 i) (L2 i)).
   Variable (sk: AST.program unit unit).
-  Hypothesis (Hsk1: linkorder (skel L1a) sk)
-             (Hsk2: linkorder (skel L1b) sk).
+  Hypothesis (Hsk: forall i, linkorder (skel (L1 i)) sk).
 
   Lemma horizontal_compose_simulation':
-    forward_simulation cc cc (SmallstepLinking_.semantics L1 sk)
-                       (SmallstepLinking_.semantics L2 sk).
+    forward_simulation cc cc (SmallstepLinking_.semantics' L1 sk)
+                       (SmallstepLinking_.semantics' L2 sk).
   Proof.
-    destruct HL1 as [Ha]. destruct HL2 as [Hb].
-    assert (HL: forall i, fsim_components cc cc (L1 i) (L2 i)) by (intros [|]; auto).
+    assert (HL: forall i, fsim_components cc cc (L1 i) (L2 i)).
+    {
+      intros i. specialize (H i).
+      apply epsilon. auto. exact (fun _ => True).
+    }
     constructor.
     eapply Forward_simulation with
         (SmallstepLinking_.order cc L1 L2 HL)
         (SmallstepLinking_.match_states cc L1 L2 HL).
     - reflexivity.
-    - intros i. cbn. destruct Ha, Hb.
-      rewrite fsim_footprint, fsim_footprint0. reflexivity.
+    - intros id.
+      split; intros [i Hi]; exists i; rewrite (fsim_footprint (HL i)) in *; auto.
     - intros se1 se2 w qset Hse Hse1.
       eapply SmallstepLinking_.semantics_simulation; eauto.
-      intros [|]; cbn; eapply Genv.valid_for_linkorder; eauto.
+      intros; eapply Genv.valid_for_linkorder; eauto.
     - clear - HL. intros [i x].
       induction (fsim_order_wf (HL i) x) as [x Hx IHx].
       constructor. intros z Hxz. inv Hxz; SmallstepLinking_.subst_dep. eauto.
   Qed.
+
 End HCOMP_FSIM.
+
+(* Section HCOMP_FSIM. *)
+
+(*   Context {li1 li2} (cc: callconv li1 li2) *)
+(*           (L1a L1b: Smallstep_.semantics li1 li1) *)
+(*           (L2a L2b: Smallstep_.semantics li2 li2). *)
+(*   Hypothesis (HL1: forward_simulation cc cc L1a L2a) *)
+(*              (HL2: forward_simulation cc cc L1b L2b). *)
+(*   Let L1 := fun b => match b with | true => L1a | false => L1b end. *)
+(*   Let L2 := fun b => match b with | true => L2a | false => L2b end. *)
+
+(*   Variable (sk: AST.program unit unit). *)
+(*   Hypothesis (Hsk1: linkorder (skel L1a) sk) *)
+(*              (Hsk2: linkorder (skel L1b) sk). *)
+
+(*   Lemma horizontal_compose_simulation': *)
+(*     forward_simulation cc cc (SmallstepLinking_.semantics L1 sk) *)
+(*                        (SmallstepLinking_.semantics L2 sk). *)
+(*   Proof. *)
+(*     destruct HL1 as [Ha]. destruct HL2 as [Hb]. *)
+(*     assert (HL: forall i, fsim_components cc cc (L1 i) (L2 i)) by (intros [|]; auto). *)
+(*     constructor. *)
+(*     eapply Forward_simulation with *)
+(*         (SmallstepLinking_.order cc L1 L2 HL) *)
+(*         (SmallstepLinking_.match_states cc L1 L2 HL). *)
+(*     - reflexivity. *)
+(*     - intros i. cbn. destruct Ha, Hb. *)
+(*       split; (intros [[|] ?]; [exists true | exists false]); cbn in *; firstorder. *)
+(*     - intros se1 se2 w qset Hse Hse1. *)
+(*       eapply SmallstepLinking_.semantics_simulation; eauto. *)
+(*       intros [|]; cbn; eapply Genv.valid_for_linkorder; eauto. *)
+(*     - clear - HL. intros [i x]. *)
+(*       induction (fsim_order_wf (HL i) x) as [x Hx IHx]. *)
+(*       constructor. intros z Hxz. inv Hxz; SmallstepLinking_.subst_dep. eauto. *)
+(*   Qed. *)
+(* End HCOMP_FSIM. *)
 
 Section COMP_FSIM.
 
@@ -96,150 +132,150 @@ Section COMP_FSIM.
 
 End COMP_FSIM.
 
-Require Import SmallstepLinking_.
+(* Require Import SmallstepLinking_. *)
 
-Section HCOMP_ASSOC.
+(* Section HCOMP_ASSOC. *)
 
-  Context {li} (L1 L2 L3: Smallstep_.semantics li li).
-  Variable (sk: AST.program unit unit).
-  Let L12 := fun b => match b with | true => L1 | false => L2 end.
-  Let L := fun b => match b with
-                 | true => SmallstepLinking_.semantics L12 sk
-                 | false => L3
-                 end.
-  Let L23 := fun b => match b with | true => L2 | false => L3 end.
-  Let L' := fun b => match b with
-                  | true => L1
-                  | false => SmallstepLinking_.semantics L23 sk
-                  end.
+(*   Context {li} (L1 L2 L3: Smallstep_.semantics li li). *)
+(*   Variable (sk: AST.program unit unit). *)
+(*   Let L12 := fun b => match b with | true => L1 | false => L2 end. *)
+(*   Let L := fun b => match b with *)
+(*                  | true => SmallstepLinking_.semantics L12 sk *)
+(*                  | false => L3 *)
+(*                  end. *)
+(*   Let L23 := fun b => match b with | true => L2 | false => L3 end. *)
+(*   Let L' := fun b => match b with *)
+(*                   | true => L1 *)
+(*                   | false => SmallstepLinking_.semantics L23 sk *)
+(*                   end. *)
 
-  Variant frame3: Type :=
-  | fm1: state L1 -> frame3
-  | fm2: state L2 -> frame3
-  | fm3: state L3 -> frame3.
+(*   Variant frame3: Type := *)
+(*   | fm1: state L1 -> frame3 *)
+(*   | fm2: state L2 -> frame3 *)
+(*   | fm3: state L3 -> frame3. *)
 
-  Inductive flatten1: list (frame L) -> list frame3 -> Prop :=
-  | flatten1_nil_nil: flatten1 nil nil
-  | flatten1_fm1' s k2 k:
-      flatten1 k2 k ->
-      flatten1 (st L true (st L12 true s :: nil) :: k2) (fm1 s :: k)
-  | flatten1_fm1 s k1 k2 k:
-      k1 <> nil -> flatten1 (st L true k1 :: k2) k ->
-      flatten1 (st L true (st L12 true s :: k1) :: k2) (fm1 s :: k)
-  | flatten1_fm2' s k2 k:
-      flatten1 k2 k ->
-      flatten1 (st L true (st L12 false s :: nil) :: k2) (fm2 s :: k)
-  | flatten1_fm2 s k1 k2 k:
-      k1 <> nil -> flatten1 (st L true k1 :: k2) k ->
-      flatten1 (st L true (st L12 false s :: k1) :: k2) (fm2 s :: k)
-  | flatten1_fm3 s k1 k:
-      flatten1 k1 k ->
-      flatten1 (st L false s :: k1) (fm3 s :: k).
+(*   Inductive flatten1: list (frame L) -> list frame3 -> Prop := *)
+(*   | flatten1_nil_nil: flatten1 nil nil *)
+(*   | flatten1_fm1' s k2 k: *)
+(*       flatten1 k2 k -> *)
+(*       flatten1 (st L true (st L12 true s :: nil) :: k2) (fm1 s :: k) *)
+(*   | flatten1_fm1 s k1 k2 k: *)
+(*       k1 <> nil -> flatten1 (st L true k1 :: k2) k -> *)
+(*       flatten1 (st L true (st L12 true s :: k1) :: k2) (fm1 s :: k) *)
+(*   | flatten1_fm2' s k2 k: *)
+(*       flatten1 k2 k -> *)
+(*       flatten1 (st L true (st L12 false s :: nil) :: k2) (fm2 s :: k) *)
+(*   | flatten1_fm2 s k1 k2 k: *)
+(*       k1 <> nil -> flatten1 (st L true k1 :: k2) k -> *)
+(*       flatten1 (st L true (st L12 false s :: k1) :: k2) (fm2 s :: k) *)
+(*   | flatten1_fm3 s k1 k: *)
+(*       flatten1 k1 k -> *)
+(*       flatten1 (st L false s :: k1) (fm3 s :: k). *)
 
-  Inductive flatten2: list (frame L') -> list frame3 -> Prop :=
-  | flatten2_nil_nil: flatten2 nil nil
-  | flatten2_fm1 s k1 k:
-      flatten2 k1 k ->
-      flatten2 (st L' true s :: k1) (fm1 s :: k)
-  | flatten2_fm2' s k2 k:
-      flatten2 k2 k ->
-      flatten2 (st L' false (st L23 true s :: nil) :: k2) (fm2 s :: k)
-  | flatten2_fm2 s k1 k2 k:
-      k1 <> nil -> flatten2 (st L' false k1 :: k2) k ->
-      flatten2 (st L' false (st L23 true s :: k1) :: k2) (fm2 s :: k)
-  | flatten2_fm3' s k2 k:
-      flatten2 k2 k ->
-      flatten2 (st L' false (st L23 false s :: nil) :: k2) (fm3 s :: k)
-  | flatten2_fm3 s k1 k2 k:
-      k1 <> nil -> flatten2 (st L' false k1 :: k2) k ->
-      flatten2 (st L' false (st L23 false s :: k1) :: k2) (fm3 s :: k).
+(*   Inductive flatten2: list (frame L') -> list frame3 -> Prop := *)
+(*   | flatten2_nil_nil: flatten2 nil nil *)
+(*   | flatten2_fm1 s k1 k: *)
+(*       flatten2 k1 k -> *)
+(*       flatten2 (st L' true s :: k1) (fm1 s :: k) *)
+(*   | flatten2_fm2' s k2 k: *)
+(*       flatten2 k2 k -> *)
+(*       flatten2 (st L' false (st L23 true s :: nil) :: k2) (fm2 s :: k) *)
+(*   | flatten2_fm2 s k1 k2 k: *)
+(*       k1 <> nil -> flatten2 (st L' false k1 :: k2) k -> *)
+(*       flatten2 (st L' false (st L23 true s :: k1) :: k2) (fm2 s :: k) *)
+(*   | flatten2_fm3' s k2 k: *)
+(*       flatten2 k2 k -> *)
+(*       flatten2 (st L' false (st L23 false s :: nil) :: k2) (fm3 s :: k) *)
+(*   | flatten2_fm3 s k1 k2 k: *)
+(*       k1 <> nil -> flatten2 (st L' false k1 :: k2) k -> *)
+(*       flatten2 (st L' false (st L23 false s :: k1) :: k2) (fm3 s :: k). *)
 
-  Hint Constructors flatten1 flatten2.
+(*   Hint Constructors flatten1 flatten2. *)
 
-  Definition state_match (s1: list (frame L)) (s2: list (frame L')): Prop :=
-    exists fm, flatten1 s1 fm /\ flatten2 s2 fm.
+(*   Definition state_match (s1: list (frame L)) (s2: list (frame L')): Prop := *)
+(*     exists fm, flatten1 s1 fm /\ flatten2 s2 fm. *)
 
-  Lemma horizontal_compose_associativity:
-    SmallstepLinking_.semantics L sk ≤ SmallstepLinking_.semantics L' sk.
-  Proof.
-    constructor. econstructor. reflexivity.
-    intros. apply or_assoc.
-    intros se ? [ ] qset [ ] Hse.
-    instantiate (1 := fun _ _ _ => _). cbn beta.
-    apply forward_simulation_step
-      with (match_states := state_match); cbn.
-    - intros q ? s1 <- H. inv H. destruct i.
-      (* initial state of L12 *)
-      + cbn in *. inv H1. destruct i.
-        (* initial state of L1 *)
-        * cbn in *. eexists; split.
-          apply initial_state_intro with (i := true).
-          firstorder. eauto.
-          eexists. split; eauto.
-        (* initial state of L2 *)
-        * cbn in *. eexists; split.
-          apply initial_state_intro with (i := false).
-          cbn. firstorder.
-          apply initial_state_intro with (i := true).
-          firstorder. eauto.
-          eexists. split; eauto.
-      (* initial state of L3 *)
-      + cbn in *. eexists; split.
-        apply initial_state_intro with (i := false).
-        cbn. firstorder.
-        apply initial_state_intro with (i := false).
-        firstorder. eauto.
-        eexists. split; eauto.
-    - intros s1 s2 r Hs H. exists r; split; auto.
-      inv H. destruct i.
-      (* final state of L12 *)
-      + cbn in *. inv H0. destruct i.
-        (* final state of L1 *)
-        * cbn in *. destruct Hs as [fs [Hs1 Hs2]].
-          admit.
-        (* final state of L2 *)
-        * admit.
-      (* final state of L3 *)
-      + cbn in *. destruct Hs as [fs [Hs1 Hs2]].
-        inv Hs1. subst_dep.
-        inv H3. inv Hs2. inv H2.
-        repeat constructor; auto.
-        inv H4.
-    - admit.
-    - intros s1 t s1' Hstep s2 Hs.
-      inv Hstep.
-      (* internal step *)
-      + destruct i.
-        (* internal step of L12 *)
-        * inv H.
-          (* internal step of L1 or L2 *)
-          {
-            destruct i.
-            (* internal step of L1 *)
-            - destruct Hs as [fm [Hs1 Hs2]].
-              admit.
-            (* internal step of L2 *)
-            - admit.
-          }
-          (* cross component call between L1 and L2 *)
-          -- admit.
-          (* return *)
-          -- admit.
-        (* internal step of L3 *)
-        * admit.
-      (* cross component call between L12 and L3 *)
-      + destruct i.
-        (* call from L12 *)
-        * cbn in *. inv H. destruct i.
-          (* call from L1 *)
-          -- admit.
-          (* call from L2 *)
-          -- admit.
-        (* call from L3 *)
-        * admit.
-      (* return *)
-      + admit.
+(*   Lemma horizontal_compose_associativity: *)
+(*     SmallstepLinking_.semantics L sk ≤ SmallstepLinking_.semantics L' sk. *)
+(*   Proof. *)
+(*     constructor. econstructor. reflexivity. *)
+(*     intros. apply or_assoc. *)
+(*     intros se ? [ ] qset [ ] Hse. *)
+(*     instantiate (1 := fun _ _ _ => _). cbn beta. *)
+(*     apply forward_simulation_step *)
+(*       with (match_states := state_match); cbn. *)
+(*     - intros q ? s1 <- H. inv H. destruct i. *)
+(*       (* initial state of L12 *) *)
+(*       + cbn in *. inv H1. destruct i. *)
+(*         (* initial state of L1 *) *)
+(*         * cbn in *. eexists; split. *)
+(*           apply initial_state_intro with (i := true). *)
+(*           firstorder. eauto. *)
+(*           eexists. split; eauto. *)
+(*         (* initial state of L2 *) *)
+(*         * cbn in *. eexists; split. *)
+(*           apply initial_state_intro with (i := false). *)
+(*           cbn. firstorder. *)
+(*           apply initial_state_intro with (i := true). *)
+(*           firstorder. eauto. *)
+(*           eexists. split; eauto. *)
+(*       (* initial state of L3 *) *)
+(*       + cbn in *. eexists; split. *)
+(*         apply initial_state_intro with (i := false). *)
+(*         cbn. firstorder. *)
+(*         apply initial_state_intro with (i := false). *)
+(*         firstorder. eauto. *)
+(*         eexists. split; eauto. *)
+(*     - intros s1 s2 r Hs H. exists r; split; auto. *)
+(*       inv H. destruct i. *)
+(*       (* final state of L12 *) *)
+(*       + cbn in *. inv H0. destruct i. *)
+(*         (* final state of L1 *) *)
+(*         * cbn in *. destruct Hs as [fs [Hs1 Hs2]]. *)
+(*           admit. *)
+(*         (* final state of L2 *) *)
+(*         * admit. *)
+(*       (* final state of L3 *) *)
+(*       + cbn in *. destruct Hs as [fs [Hs1 Hs2]]. *)
+(*         inv Hs1. subst_dep. *)
+(*         inv H3. inv Hs2. inv H2. *)
+(*         repeat constructor; auto. *)
+(*         inv H4. *)
+(*     - admit. *)
+(*     - intros s1 t s1' Hstep s2 Hs. *)
+(*       inv Hstep. *)
+(*       (* internal step *) *)
+(*       + destruct i. *)
+(*         (* internal step of L12 *) *)
+(*         * inv H. *)
+(*           (* internal step of L1 or L2 *) *)
+(*           { *)
+(*             destruct i. *)
+(*             (* internal step of L1 *) *)
+(*             - destruct Hs as [fm [Hs1 Hs2]]. *)
+(*               admit. *)
+(*             (* internal step of L2 *) *)
+(*             - admit. *)
+(*           } *)
+(*           (* cross component call between L1 and L2 *) *)
+(*           -- admit. *)
+(*           (* return *) *)
+(*           -- admit. *)
+(*         (* internal step of L3 *) *)
+(*         * admit. *)
+(*       (* cross component call between L12 and L3 *) *)
+(*       + destruct i. *)
+(*         (* call from L12 *) *)
+(*         * cbn in *. inv H. destruct i. *)
+(*           (* call from L1 *) *)
+(*           -- admit. *)
+(*           (* call from L2 *) *)
+(*           -- admit. *)
+(*         (* call from L3 *) *)
+(*         * admit. *)
+(*       (* return *) *)
+(*       + admit. *)
 
-  Admitted.
+(*   Admitted. *)
 
-End HCOMP_ASSOC.
+(* End HCOMP_ASSOC. *)
